define general forward simulation where the source language is kept abstract and Boogie is the target language, define general structural rules on this simulation
stmt_rel_seq, stmt_rel_if, inhale_seq are now proved by using the general structural rules

InhaleRel.thy
@@ -1,5 +1,5 @@
 theory InhaleRel
-  imports ExpRel ExprWfRel TotalViper.ViperBoogieTranslationInterface
+  imports ExpRel ExprWfRel TotalViper.ViperBoogieTranslationInterface StmtRel
 begin
 
 definition inhale_rel ::
@@ -11,15 +11,11 @@ definition inhale_rel ::
                        \<Rightarrow> (pure_exp, pure_exp atomic_assert) assert
                           \<Rightarrow> bigblock \<times> cont \<Rightarrow> bigblock \<times> cont \<Rightarrow> bool"
   where "inhale_rel R ctxt_vpr StateCons P ctxt assertion_vpr \<gamma> \<gamma>' \<equiv>
-           \<forall>\<omega> ns res. R \<omega> ns \<longrightarrow> 
-             \<comment>\<open>If the Viper inhale reduces\<close>
-             red_inhale ctxt_vpr StateCons assertion_vpr \<omega> res \<longrightarrow>
-             (\<forall>\<omega>'. res = RNormal \<omega>' \<longrightarrow>
-                   \<comment>\<open>Normal Viper inhale executions can be simulated by normal Boogie executions\<close>
-                   (\<exists>ns'. (red_ast_bpl P ctxt (\<gamma>, Normal ns) (\<gamma>', Normal ns') \<and> R \<omega>' ns'))) \<and>
-             (res = RFailure \<longrightarrow> 
-                   \<comment>\<open>If a Viper inhale executions fails, then there is a failing Boogie execution\<close>
-                   (\<exists>c'. red_ast_bpl P ctxt (\<gamma>, Normal ns) c' \<and> snd c' = Failure))"
+         rel_general R R 
+           (\<lambda> \<omega> \<omega>'. red_inhale ctxt_vpr StateCons assertion_vpr \<omega> (RNormal \<omega>'))
+           (\<lambda> \<omega>. red_inhale ctxt_vpr StateCons assertion_vpr \<omega> RFailure)
+           P ctxt \<gamma> \<gamma>'"
+
 
 lemma inhale_rel_intro:
   assumes
@@ -28,14 +24,14 @@ lemma inhale_rel_intro:
       red_inhale ctxt_vpr StateCons assertion_vpr \<omega> (RNormal \<omega>') \<Longrightarrow>
       (\<exists>ns'. (red_ast_bpl P ctxt (\<gamma>, Normal ns) (\<gamma>', Normal ns') \<and> R \<omega>' ns'))" and
 
-    "\<And>\<omega> ns \<omega>'.
+    "\<And>\<omega> ns.
       R \<omega> ns \<Longrightarrow>
       red_inhale ctxt_vpr StateCons assertion_vpr \<omega> RFailure \<Longrightarrow>
       (\<exists>c'. red_ast_bpl P ctxt (\<gamma>, Normal ns) c' \<and> snd c' = Failure)"
   shows "inhale_rel R ctxt_vpr StateCons P ctxt assertion_vpr \<gamma> \<gamma>'"
   using assms
   unfolding inhale_rel_def
-  by blast
+  by (auto intro: rel_intro)
 
 definition inhale_rel_aux
   where "inhale_rel_aux R ctxt_vpr StateCons P ctxt assertion_vpr \<gamma> \<gamma>' \<omega> ns res \<equiv>
@@ -55,7 +51,7 @@ lemma inhale_rel_intro_2:
   shows "inhale_rel R ctxt_vpr StateCons P ctxt assertion_vpr \<gamma> \<gamma>'"
   using assms
   unfolding inhale_rel_def inhale_rel_aux_def
-  by fastforce
+  by (auto intro: rel_intro)
 
 lemma inhale_rel_aux_intro:
   assumes "\<And>\<omega>'. res = RNormal \<omega>' \<Longrightarrow>
@@ -73,7 +69,7 @@ lemma inhale_rel_normal_elim:
   shows "\<exists>ns'. (red_ast_bpl P ctxt (\<gamma>, Normal ns) (\<gamma>', Normal ns') \<and> R \<omega>' ns')"
   using assms
   unfolding inhale_rel_def
-  by blast
+  by (auto intro: rel_success_elim)
 
 lemma inhale_rel_failure_elim:
   assumes "inhale_rel R ctxt_vpr StateCons P ctxt assertion_vpr \<gamma> \<gamma>'" and 
@@ -81,56 +77,19 @@ lemma inhale_rel_failure_elim:
           "red_inhale ctxt_vpr StateCons assertion_vpr \<omega> RFailure"
   shows "\<exists>c'. red_ast_bpl P ctxt (\<gamma>, Normal ns) c' \<and> snd c' = Failure"
   using assms
-  unfolding inhale_rel_def
-  by blast
+  unfolding inhale_rel_def rel_general_def
+  by auto
 
 subsection \<open>Structural rules\<close>
 
 lemma inhale_rel_star: 
   assumes "inhale_rel R ctxt_vpr StateCons P ctxt A1 \<gamma>1 \<gamma>2" and
           "inhale_rel R ctxt_vpr StateCons P ctxt A2 \<gamma>2 \<gamma>3"
-  shows "inhale_rel R ctxt_vpr StateCons P ctxt (A1 && A2) \<gamma>1 \<gamma>3"
-proof (rule inhale_rel_intro)
-\<comment>\<open>Normal case\<close>
-
-  fix \<omega> ns \<omega>'
-  assume "R \<omega> ns" and "red_inhale ctxt_vpr StateCons (A1 && A2) \<omega> (RNormal \<omega>')"
-  from this obtain \<omega>'' where
-    RedInhA1: "red_inhale ctxt_vpr StateCons A1 \<omega> (RNormal \<omega>'')" and
-    RedInhA2: "red_inhale ctxt_vpr StateCons A2 \<omega>'' (RNormal \<omega>')"
-    by (auto elim: InhStar_case)
-
-  from inhale_rel_normal_elim[OF assms(1) \<open>R \<omega> ns\<close> RedInhA1]
-       inhale_rel_normal_elim[OF assms(2) _ RedInhA2]
-
-  show "\<exists>ns'. red_ast_bpl P ctxt (\<gamma>1, Normal ns) (\<gamma>3, Normal ns') \<and> R \<omega>' ns'"
-    using red_ast_bpl_transitive
-    by blast
-next
-\<comment>\<open>Failure case\<close>
-
-  fix \<omega> ns \<omega>'
-  assume "R \<omega> ns" and RedInhale: "red_inhale ctxt_vpr StateCons (A1 && A2) \<omega> RFailure"
-
-  show "\<exists>c'. red_ast_bpl P ctxt (\<gamma>1, Normal ns) c' \<and> snd c' = Failure"
-  proof (cases "red_inhale ctxt_vpr StateCons A1 \<omega> RFailure")
-    case True
-    thus ?thesis 
-      using inhale_rel_failure_elim[OF assms(1) \<open>R \<omega> ns\<close>]
-      by blast
-  next
-    case False
-    with RedInhale obtain \<omega>'' where 
-      "red_inhale ctxt_vpr StateCons A1 \<omega> (RNormal \<omega>'')" and
-     "red_inhale ctxt_vpr StateCons A2 \<omega>'' RFailure"
-      by (auto elim: InhStar_case)
-
-    thus ?thesis
-      using inhale_rel_normal_elim[OF assms(1) \<open>R \<omega> ns\<close>] inhale_rel_failure_elim[OF assms(2)] 
-            red_ast_bpl_transitive
-      by fast
-  qed
-qed
+        shows "inhale_rel R ctxt_vpr StateCons P ctxt (A1 && A2) \<gamma>1 \<gamma>3"
+  using assms
+  unfolding inhale_rel_def
+  apply (rule rel_general_comp)
+  by (auto elim: InhStar_case)
 
 lemma inhale_rel_imp:
   assumes 
@@ -216,21 +175,126 @@ subsection \<open>Field access predicate rule\<close>
 
 
 lemma inhale_rel_field_acc:
-  assumes "expr_wf_rel (state_rel_ext R) ctxt_vpr StateCons P ctxt e_rcv_vpr \<gamma> \<gamma>2" and
-          "expr_wf_rel (state_rel_ext R) ctxt_vpr StateCons P ctxt e_p \<gamma>2 \<gamma>3" and
-          "wf_rel (state_rel_ext R)
+  assumes 
+    MaskUpdWf: "mask_update_wf TyRep ctxt mask_upd_bpl" and
+    WfRcv: "expr_wf_rel (state_rel_ext R) ctxt_vpr StateCons P ctxt e_rcv_vpr \<gamma> \<gamma>1" and
+    WfPerm: "expr_wf_rel (state_rel_ext R) ctxt_vpr StateCons P ctxt e_p \<gamma>1 \<gamma>2" and
+    WfInh:  "wf_rel (state_rel_ext R)
                   Rext' 
                   (\<lambda> \<omega>def \<omega>. \<exists>p r. ctxt_vpr, StateCons, Some \<omega>def \<turnstile> \<langle>e_p;\<omega>\<rangle> [\<Down>]\<^sub>t (Val (VPerm p)) \<and> p \<ge> 0 \<and>
-                                   ctxt_vpr, StateCons, Some \<omega>def \<turnstile> \<langle>e_rcv_vpr;\<omega>\<rangle> [\<Down>]\<^sub>t (Val (VRef r)) \<and> (p > 0 \<longrightarrow> r = Null))  
+                                   ctxt_vpr, StateCons, Some \<omega>def \<turnstile> \<langle>e_rcv_vpr;\<omega>\<rangle> [\<Down>]\<^sub>t (Val (VRef r)) \<and> (p > 0 \<longrightarrow> r \<noteq> Null))  
                   (\<lambda> \<omega>def \<omega>. \<exists>p. ctxt_vpr, StateCons, Some \<omega>def \<turnstile> \<langle>e_p;\<omega>\<rangle> [\<Down>]\<^sub>t (Val (VPerm p)) \<and> p < 0)
-                  P ctxt \<gamma>3 ((BigBlock name ((Lang.Assign m_bpl m_upd_bpl)#cs) str tr), cont)" and
-                   "m_bpl = mask_var Tr" and
-    HeapUpdateBpl: "m_upd_bpl = mask_update Tr (Lang.Var m_bpl) e_rcv_bpl e_f_bpl new_perm_bpl [TConSingle (TNormalFieldId TyRep), \<tau>_bpl]" and    
+                  P ctxt \<gamma>2 \<gamma>3" and
+            "m_bpl = mask_var Tr" and
+    MaskUpdBpl:
+       "\<And> \<omega> ns. Rext' \<omega> \<omega> ns \<Longrightarrow> \<exists> ns'. red_ast_bpl P ctxt (\<gamma>, Normal ns) (\<gamma>', Normal ns')" and
+    HeapUpdateBpl: "m_upd_bpl = mask_upd_bpl (Lang.Var m_bpl) e_rcv_bpl e_f_bpl new_perm_bpl [TConSingle (TNormalFieldId TyRep), \<tau>_bpl]" and    
     RcvRel: "exp_rel_vpr_bpl Rext' ctxt_vpr ctxt e_rcv_vpr rcv_bpl" and
     FieldRelSingle: "field_rel_single (program_total ctxt_vpr) TyRep Tr f_vpr e_f_bpl \<tau>_bpl" and
     NewPermRel: "exp_rel_vpr_bpl Rext' ctxt_vpr ctxt (ViperLang.Binop (Perm e_rcv_vpr f) ViperLang.Add e_p) new_perm_bpl" 
+
+    (*
+     \<comment>\<open>Inhale property for R\<close>
+    RInhale:  "\<And> \<omega> ns ty_vpr hb r f_bpl p. Rext' \<omega> \<omega> ns \<Longrightarrow>
+                     declared_fields (program_total ctxt_vpr) f_vpr = Some ty_vpr \<Longrightarrow>
+                     field_translation Tr f_vpr = Some f_bpl \<Longrightarrow>
+                     vpr_to_bpl_ty TyRep ty_vpr = Some \<tau>_bpl \<Longrightarrow>
+                     (pgt p pnone  \<Longrightarrow> r \<noteq> Null) \<Longrightarrow>
+                     (\<exists>mb f_bpl_val. 
+                       lookup_var_ty (var_context ctxt) (mask_var Tr) = Some (TConSingle (TMaskId TyRep)) \<and>
+                       lookup_var (var_context ctxt) ns (mask_var Tr) = Some (AbsV (AMask mb)) \<and>
+                       lookup_var (var_context ctxt) ns f_bpl = Some (AbsV (AField f_bpl_val)) \<and>
+                       field_ty_fun_opt TyRep f_bpl_val = Some ((TFieldId TyRep), [TConSingle (TNormalFieldId TyRep), \<tau>_bpl]) \<and>
+                       Rext'
+                         (if r = Null then \<omega> else update_mh_loc_total_full \<omega> (the_address r, f_vpr) p)
+                         (if r = Null then \<omega> else update_mh_loc_total_full \<omega> (the_address r, f_vpr) p)
+                         (update_var (var_context ctxt) ns (heap_var Tr) 
+                               (AbsV (AMask (mb ( (r, f_bpl_val) := real_of_rat (Rep_prat p) ))))
+                         ))"*)
     
   shows "inhale_rel R ctxt_vpr StateCons P ctxt (Atomic (Acc e_rcv_vpr f (PureExp e_p))) \<gamma> \<gamma>'"
-  oops
+proof (rule inhale_rel_intro_2)
+  fix \<omega> ns res
+  assume "R \<omega> ns"
+  hence Rext0: "state_rel_ext R \<omega> \<omega> ns"
+    by simp
+
+  assume "red_inhale ctxt_vpr StateCons (Atomic (Acc e_rcv_vpr f (PureExp e_p))) \<omega> res"
+  thus "inhale_rel_aux R ctxt_vpr StateCons P ctxt (Atomic (Acc e_rcv_vpr f (PureExp e_p))) \<gamma> \<gamma>' \<omega> ns res"
+  proof (cases)
+    case (InhAcc r p W')
+    from this obtain ns1 where Rext1: "state_rel_ext R \<omega> \<omega> ns1" and "red_ast_bpl P ctxt (\<gamma>, Normal ns) (\<gamma>1, Normal ns1)"
+      using wf_rel_normal_elim[OF WfRcv Rext0]
+      by blast
+    with InhAcc obtain ns2 where Rext2: "state_rel_ext R \<omega> \<omega> ns2" and Red2: "red_ast_bpl P ctxt (\<gamma>, Normal ns) (\<gamma>2, Normal ns2)"
+      using wf_rel_normal_elim[OF WfPerm Rext1] red_ast_bpl_transitive
+      by blast
+
+    show ?thesis
+    proof (rule inhale_rel_aux_intro)
+      \<comment>\<open>Normal case\<close>
+      let ?\<gamma>3 = "((BigBlock name ((Lang.Assign m_bpl m_upd_bpl)#cs) str tr), cont)"
+
+      fix \<omega>'
+      assume "res = RNormal \<omega>'"
+      hence "0 \<le> p" and "W' \<noteq> {}" and "0 < p \<longrightarrow> r \<noteq> Null" and "\<omega>' \<in> W'"
+      using th_result_rel_normal InhAcc
+      by auto
+
+      with InhAcc obtain ns3 where Rext3: "Rext' \<omega> \<omega> ns3" and "red_ast_bpl P ctxt (\<gamma>, Normal ns) (?\<gamma>3, Normal ns3)"
+        using wf_rel_normal_elim[OF WfInh Rext2] red_ast_bpl_transitive[OF Red2]
+        by blast
+
+      let ?p_bpl = "real_of_rat p"
+      let ?p_prat = "Abs_prat p"
+
+      have "pgt ?p_prat pnone  \<Longrightarrow> r \<noteq> Null"
+        using \<open>0 < p \<longrightarrow> r \<noteq> Null\<close> \<open>p \<ge> 0\<close> pnone_def prat_pgt_pnone
+        by fastforce        
+
+      obtain f_bpl \<tau>_vpr where
+          FieldLookup: "declared_fields (program_total ctxt_vpr) f_vpr = Some \<tau>_vpr" and
+          TyTr: "vpr_to_bpl_ty TyRep \<tau>_vpr = Some \<tau>_bpl" and
+          FieldTr: "field_translation Tr f_vpr = Some f_bpl" and
+          "e_f_bpl = Lang.Var f_bpl"
+        using FieldRelSingle
+        by (auto elim: field_rel_single_elim)
+
+      from Rext3 
+
+      from MaskUpdWf have
+        RedMaskUpdBpl:
+        "red_expr_bpl ctxt (mask_upd_bpl (Lang.Var m_bpl) e_rcv_bpl e_f_bpl new_perm_bpl [TConSingle (TNormalFieldId TyRep), \<tau>_bpl])
+                           ns3
+                           (AbsV (AMask (m ( (r, f_bpl_val) := ?p_bpl))))"
+       (* 
+            from HeapUpdWf have 
+            RedHeapUpdBpl:
+           "red_expr_bpl ctxt (heap_update Tr (Lang.Var h_bpl) rcv_bpl e_f_bpl rhs_bpl [TConSingle (TNormalFieldId TyRep), \<tau>_bpl])
+                                   ns3 (AbsV (AHeap (hb( (Address addr,f_bpl_val) \<mapsto> (val_rel_vpr_bpl v) ))))"
+           apply (rule heap_update_wf_apply)
+           using  \<open>h_bpl = _\<close> Semantics.RedVar[OF LookupHeapVarBpl]
+                 apply simp
+                apply (rule HeapWellTyBpl)
+               apply (rule RedRcvBpl)
+           using \<open>e_f_bpl = _\<close> Semantics.RedVar[OF LookupFieldVarBpl]
+              apply simp
+             apply (rule FieldTyBpl)
+            apply (rule RedRhsBpl)
+           apply (simp add: NewValTypeBpl)
+           done
+       *)
+        
+        
+      
+    
+    then show ?thesis sorry
+  next 
+    case InhSubAtomicFailure
+    then show ?thesis sorry
+  qed
+next
+  
+
 
 end
