Simulation.thy
@@ -1,0 +1,282 @@
+section \<open>Generic definitions for simulations between front-ends and Boogie\<close>
+
+theory Simulation
+imports BoogieInterface
+begin
+
+definition rel_general :: "('v \<Rightarrow> 'a nstate \<Rightarrow> bool) \<Rightarrow>
+                               ('v \<Rightarrow> 'a nstate \<Rightarrow> bool) \<Rightarrow> 
+                                ('v \<Rightarrow> 'v \<Rightarrow> bool) \<Rightarrow>
+                                ('v \<Rightarrow> bool) \<Rightarrow>
+                                ast \<Rightarrow> 'a econtext_bpl_general \<Rightarrow>
+                                (Ast.bigblock \<times> cont) \<Rightarrow> (Ast.bigblock \<times> cont) \<Rightarrow> bool"
+  where 
+    "rel_general R R' Success Fail P ctxt \<gamma> \<gamma>' \<equiv>
+      \<comment>\<open>for all states in the input relation\<close>
+      \<forall> \<omega> ns. R \<omega> ns \<longrightarrow> 
+             (\<forall>\<omega>'. Success \<omega> \<omega>' \<longrightarrow>
+                 \<comment>\<open>success can be simulated by an Boogie execution that reaches \<gamma>' s.t. 
+                    the output relation is respected\<close>
+                 (\<exists>ns'. (red_ast_bpl P ctxt (\<gamma>, Normal ns) (\<gamma>', Normal ns') \<and> R' \<omega>' ns'))) \<and>
+             (Fail \<omega> \<longrightarrow> 
+                 \<comment>\<open>failure is preserved by Boogie\<close>
+                (\<exists>c'. snd c' = Failure \<and>
+                      red_ast_bpl P ctxt (\<gamma>, Normal ns) c'))"
+
+subsection \<open>Introduction and Elimination rules\<close>
+
+lemma rel_intro:
+  assumes 
+  "\<And>\<omega> ns \<omega>'. 
+          R \<omega> ns \<Longrightarrow> 
+          Success \<omega> \<omega>' \<Longrightarrow>
+          \<exists>ns'. (red_ast_bpl P ctxt (\<gamma>, Normal ns) (\<gamma>', Normal ns') \<and> R' \<omega>' ns')" and
+  "\<And>\<omega> ns.
+          R \<omega> ns \<Longrightarrow> 
+          Fail \<omega> \<Longrightarrow>
+          \<exists>c'. snd c' = Failure \<and> red_ast_bpl P ctxt (\<gamma>, Normal ns) c'"
+  shows "rel_general R R' Success Fail P ctxt \<gamma> \<gamma>'"
+  using assms
+  unfolding rel_general_def 
+  by blast
+
+lemma rel_success_elim:
+  assumes "rel_general R R' Success Fail P ctxt \<gamma> \<gamma>'" and
+          "R \<omega> ns" and
+          "Success \<omega> \<omega>'"
+    shows   "\<exists>ns'. (red_ast_bpl P ctxt (\<gamma>, Normal ns) (\<gamma>', Normal ns') \<and> R' \<omega>' ns')"
+  using assms
+  unfolding rel_general_def
+  by blast
+
+lemma rel_failure_elim:
+  assumes "rel_general R R' Success Fail P ctxt \<gamma> \<gamma>'" and
+          "R \<omega> ns" and
+          "Fail \<omega>"
+  shows "\<exists>c'. snd c' = Failure \<and> red_ast_bpl P ctxt (\<gamma>, Normal ns) c'"
+  using assms
+  unfolding rel_general_def
+  by blast
+
+subsection \<open>Propagation rules\<close>
+
+lemma rel_propagate_pre:
+  assumes "\<And> \<omega> ns. R0 \<omega> ns \<Longrightarrow> \<exists>ns'. red_ast_bpl P ctxt (\<gamma>0, Normal ns) (\<gamma>1, Normal ns') \<and> R1 \<omega> ns'" and
+          "rel_general R1 R2 Success Fail P ctxt \<gamma>1 \<gamma>2"
+        shows "rel_general R0 R2 Success Fail P ctxt \<gamma>0 \<gamma>2"  
+proof (rule rel_intro)
+  fix \<omega> ns \<omega>'
+  assume "R0 \<omega> ns" and "Success \<omega> \<omega>'"
+
+  from \<open>R0 \<omega> ns\<close> and assms(1) obtain ns1 where
+    "red_ast_bpl P ctxt (\<gamma>0, Normal ns) (\<gamma>1, Normal ns1)" and "R1 \<omega> ns1"
+    by blast
+
+  thus "\<exists>ns'. red_ast_bpl P ctxt (\<gamma>0, Normal ns) (\<gamma>2, Normal ns') \<and> R2 \<omega>' ns'"
+    using rel_success_elim[OF assms(2)] \<open>Success \<omega> \<omega>'\<close>
+    by (metis (no_types, opaque_lifting) red_ast_bpl_transitive)
+next
+  fix \<omega> ns \<omega>'
+  assume "R0 \<omega> ns" and "Fail \<omega>"
+
+  from \<open>R0 \<omega> ns\<close> and assms(1) obtain ns1 where
+    "red_ast_bpl P ctxt (\<gamma>0, Normal ns) (\<gamma>1, Normal ns1)" and "R1 \<omega> ns1"
+    by blast
+
+  thus "\<exists>c'. snd c' = Failure \<and> red_ast_bpl P ctxt (\<gamma>0, Normal ns) c'"
+    using rel_failure_elim[OF assms(2)] \<open>Fail \<omega>\<close>
+    by (metis (no_types, opaque_lifting) red_ast_bpl_transitive)
+qed
+
+lemma rel_propagate_post:
+  assumes "rel_general R0 R1 Success Fail P ctxt \<gamma>0 \<gamma>1" and
+          "\<And> \<omega> ns. R1 \<omega> ns \<Longrightarrow> \<exists>ns'. red_ast_bpl P ctxt (\<gamma>1, Normal ns) (\<gamma>2, Normal ns') \<and> R2 \<omega> ns'"
+  shows "rel_general R0 R2 Success Fail P ctxt \<gamma>0 \<gamma>2"
+proof (rule rel_intro)
+  fix \<omega> ns \<omega>'
+  assume "R0 \<omega> ns" and
+         "Success \<omega> \<omega>'"  
+  from this obtain ns1 where 
+    "red_ast_bpl P ctxt (\<gamma>0, Normal ns) (\<gamma>1, Normal ns1)" and "R1 \<omega>' ns1"
+    using assms(1) rel_success_elim 
+    by metis 
+
+  thus "\<exists>ns'. red_ast_bpl P ctxt (\<gamma>0, Normal ns) (\<gamma>2, Normal ns') \<and> R2 \<omega>' ns'"
+    using assms(2)
+    by (metis (no_types, opaque_lifting) red_ast_bpl_transitive)
+next
+  fix \<omega> ns
+  assume "R0 \<omega> ns" and
+         "Fail \<omega>"
+  thus "\<exists>c'. snd c' = Failure \<and> red_ast_bpl P ctxt (\<gamma>0, Normal ns) c'"
+    using assms(1) rel_failure_elim 
+    by meson
+qed
+
+subsection \<open>General structural rules\<close>
+
+text \<open>Composition rule\<close>
+
+lemma rel_general_comp:
+  assumes 
+   Rel1: "rel_general R1 R2 Success1 Fail1 P ctxt \<gamma>1 \<gamma>2" and
+   Rel2: "rel_general R2 R3 Success2 Fail2 P ctxt \<gamma>2 \<gamma>3" and
+   SuccessComp: "\<And> \<omega> \<omega>'. Success3 \<omega> \<omega>' \<Longrightarrow> (\<exists> \<omega>''. Success1 \<omega> \<omega>'' \<and> Success2 \<omega>'' \<omega>')" and
+   FailComp: "\<And> \<omega>. Fail3 \<omega> \<Longrightarrow> (Fail1 \<omega> \<or> (\<exists>\<omega>''. Success1 \<omega> \<omega>'' \<and> Fail2 \<omega>''))"
+ shows 
+   "rel_general R1 R3 Success3 Fail3 P ctxt \<gamma>1 \<gamma>3"
+proof (rule rel_intro)
+  fix \<omega> ns \<omega>'
+  assume "R1 \<omega> ns" and "Success3 \<omega> \<omega>'"
+  with SuccessComp obtain \<omega>'' where "Success1 \<omega> \<omega>''" and "Success2 \<omega>'' \<omega>'"
+    by auto
+
+  thus "\<exists>ns'. red_ast_bpl P ctxt (\<gamma>1, Normal ns) (\<gamma>3, Normal ns') \<and> R3 \<omega>' ns'"
+    using rel_success_elim[OF Rel1 \<open>R1 \<omega> ns\<close>] rel_success_elim[OF Rel2] red_ast_bpl_transitive
+    by fast
+next
+  fix \<omega> ns
+  assume "R1 \<omega> ns" and "Fail3 \<omega>"
+
+  show "\<exists>c'. snd c' = Failure \<and> red_ast_bpl P ctxt (\<gamma>1, Normal ns) c'"
+  proof (cases "Fail1 \<omega>")
+    case True
+    then show ?thesis
+      using rel_failure_elim[OF Rel1 \<open>R1 _ _\<close>]
+      by blast
+  next
+    case False
+    with FailComp[OF \<open>Fail3 \<omega>\<close>] obtain \<omega>'' where "Success1 \<omega> \<omega>''" and "Fail2 \<omega>''"
+      by auto
+      
+    then show ?thesis
+      using rel_success_elim[OF Rel1 \<open>R1 \<omega> ns\<close>] rel_failure_elim[OF Rel2] red_ast_bpl_transitive
+      by fast
+  qed
+qed
+
+text \<open>Conditional rule\<close>
+
+lemma rel_general_cond:
+  assumes 
+          RelCondExp: "rel_general R R SuccessExp FailExp P ctxt 
+                           \<gamma> 
+                           (if_bigblock name (Some (cond_bpl)) (thn_hd # thn_tl) (els_hd # els_tl), KSeq next cont)"
+                           (is "rel_general R R SuccessExp FailExp P ctxt \<gamma> ?\<gamma>_if") and
+          RelThn: "rel_general R R SuccessThn FailThn P ctxt (thn_hd, convert_list_to_cont thn_tl (KSeq next cont)) (next, cont)" and
+          RelElse: "rel_general R R SuccessElse FailElse P ctxt (els_hd, convert_list_to_cont els_tl (KSeq next cont)) (next, cont)" and
+          SuccessCond: "\<And> \<omega> \<omega>' ns. Success \<omega> \<omega>' \<Longrightarrow> R \<omega> ns \<Longrightarrow>
+                        SuccessExp \<omega> \<omega> \<and> \<comment>\<open>implicit assumption that success of conditional does not lead to side effects\<close>
+                       ((red_expr_bpl ctxt cond_bpl ns (BoolV True) \<and> SuccessThn \<omega> \<omega>') \<or> 
+                       (red_expr_bpl ctxt cond_bpl ns (BoolV False) \<and> SuccessElse \<omega> \<omega>'))"  and
+          FailCond: "\<And> \<omega> ns. Fail \<omega> \<Longrightarrow> R \<omega> ns \<Longrightarrow> 
+               FailExp \<omega> \<or>
+               (SuccessExp \<omega> \<omega> \<and>
+                 ( (red_expr_bpl ctxt cond_bpl ns (BoolV True) \<and> FailThn \<omega>) \<or> 
+                   (red_expr_bpl ctxt cond_bpl ns (BoolV False) \<and> FailElse \<omega>) )
+               )" 
+        shows "rel_general R R Success Fail P ctxt \<gamma> (next, cont)"
+proof (rule rel_intro)
+  fix \<omega> ns \<omega>'
+  assume "R \<omega> ns" and "Success \<omega> \<omega>'"
+  have "SuccessExp \<omega> \<omega>"
+    using SuccessCond[OF \<open>Success \<omega> \<omega>'\<close> \<open>R \<omega> ns\<close>]
+    by simp
+
+  with rel_success_elim[OF RelCondExp \<open>R \<omega> ns\<close>]  
+  obtain ns1 where RedToIf: "red_ast_bpl P ctxt (\<gamma>, Normal ns) (?\<gamma>_if, Normal ns1)" and "R \<omega> ns1"
+    by blast
+
+  have Branch: "(red_expr_bpl ctxt cond_bpl ns1 (BoolV True) \<and> SuccessThn \<omega> \<omega>') \<or> 
+                (red_expr_bpl ctxt cond_bpl ns1 (BoolV False) \<and> SuccessElse \<omega> \<omega>')" 
+                            (is "?thn_branch \<or> ?els_branch")
+    using SuccessCond[OF \<open>Success \<omega> \<omega>'\<close> \<open>R \<omega> ns1\<close>]
+    by simp
+
+  show "\<exists>ns'. red_ast_bpl P ctxt (\<gamma>, Normal ns) ((next, cont), Normal ns') \<and> R \<omega>' ns'"
+  proof (cases ?thn_branch)
+    case True
+    hence "SuccessThn \<omega> \<omega>'" by simp
+
+    have "red_ast_bpl P ctxt (?\<gamma>_if, Normal ns1) ((thn_hd, convert_list_to_cont thn_tl (KSeq next cont)), Normal ns1)"
+      apply (rule red_ast_bpl_one_step_empty_simple_cmd)
+      apply (rule RedParsedIfTrue)
+      using True by blast
+
+    then show ?thesis 
+      using RedToIf rel_success_elim[OF RelThn \<open>R \<omega> ns1\<close> \<open>SuccessThn \<omega> \<omega>'\<close>] red_ast_bpl_transitive
+      by blast
+  next
+    case False
+    hence RedExpFalse:"red_expr_bpl ctxt cond_bpl ns1 (BoolV False)" and "SuccessElse \<omega> \<omega>'" using Branch
+      by auto
+
+    have "red_ast_bpl P ctxt (?\<gamma>_if, Normal ns1) ((els_hd, convert_list_to_cont els_tl (KSeq next cont)), Normal ns1)"
+      apply (rule red_ast_bpl_one_step_empty_simple_cmd)
+      apply (rule RedParsedIfFalse)
+      using RedExpFalse by blast
+
+    then show ?thesis
+      using RedToIf rel_success_elim[OF RelElse \<open>R \<omega> ns1\<close> \<open>SuccessElse \<omega> \<omega>'\<close>] red_ast_bpl_transitive
+      by blast
+  qed
+next
+  fix \<omega> ns
+  assume "R \<omega> ns" and "Fail \<omega>"
+  hence FailBranch: "FailExp \<omega> \<or> SuccessExp \<omega> \<omega>" 
+    using FailCond
+    by blast
+
+  show "\<exists>c'. snd c' = Failure \<and> red_ast_bpl P ctxt (\<gamma>, Normal ns) c'"
+  proof (cases "FailExp \<omega>")
+    case True
+    then show ?thesis 
+      using rel_failure_elim[OF RelCondExp \<open>R \<omega> ns\<close>] 
+      by blast
+  next
+    case False
+    hence "SuccessExp \<omega> \<omega>"
+      using FailBranch
+      by auto
+
+    with rel_success_elim[OF RelCondExp \<open>R \<omega> ns\<close>]  
+    obtain ns1 where RedToIf: "red_ast_bpl P ctxt (\<gamma>, Normal ns) (?\<gamma>_if, Normal ns1)" and "R \<omega> ns1"
+      by blast
+
+    hence FailBranch2: "( (red_expr_bpl ctxt cond_bpl ns1 (BoolV True) \<and> FailThn \<omega>) \<or> 
+                   (red_expr_bpl ctxt cond_bpl ns1 (BoolV False) \<and> FailElse \<omega>) )" (is "?thn_branch \<or> ?els_branch")
+      using FailCond[OF \<open>Fail \<omega>\<close>] False
+      by blast      
+
+    show ?thesis
+    proof (cases ?thn_branch)
+      case True
+      hence "FailThn \<omega>"
+        by simp
+
+      have "red_ast_bpl P ctxt (?\<gamma>_if, Normal ns1) ((thn_hd, convert_list_to_cont thn_tl (KSeq next cont)), Normal ns1)"
+      apply (rule red_ast_bpl_one_step_empty_simple_cmd)
+      apply (rule RedParsedIfTrue)
+      using True by blast
+      then show ?thesis 
+        using RedToIf rel_failure_elim[OF RelThn \<open>R \<omega> ns1\<close> \<open>FailThn \<omega>\<close>] red_ast_bpl_transitive
+        by blast
+    next
+      case False
+      hence RedExpFalse: "red_expr_bpl ctxt cond_bpl ns1 (BoolV False)" and "FailElse \<omega>"
+        using FailBranch2
+        by auto
+
+      have "red_ast_bpl P ctxt (?\<gamma>_if, Normal ns1) ((els_hd, convert_list_to_cont els_tl (KSeq next cont)), Normal ns1)"
+      apply (rule red_ast_bpl_one_step_empty_simple_cmd)
+      apply (rule RedParsedIfFalse)
+      using RedExpFalse by blast
+      then show ?thesis 
+        using RedToIf rel_failure_elim[OF RelElse \<open>R \<omega> ns1\<close> \<open>FailElse \<omega>\<close>] red_ast_bpl_transitive
+        by blast
+    qed
+  qed
+qed
+    
+
+end
